theories/typing/cont_context.v
@@ -1,4 +1,6 @@
-From lrust.typing Require Export type_context.
+From iris.proofmode Require Import tactics.
+From lrust.lang Require Import notation.
+From lrust.typing Require Import type lft_contexts type_context.
 Set Default Proof Using "Type".
 
 Section cont_context.
