theories/typing/uniq_bor.v
@@ -14,7 +14,7 @@ Section uniq_bor.
     ty_size := 1;  ty_lfts := κ :: ty.(ty_lfts);  ty_E := ty.(ty_E) ++ ty_outlv_E ty κ;
     ty_own vπ d tid vl := κ ⊑ ty.(ty_lft) ∗ [loc[l] := vl] ∃d' i,
       let ξ := PrVar (𝔄 ↾ prval_to_inh' vπ) i in
-      ⌜S d' ≤ d ∧ snd ∘ vπ = (.$ ξ)⌝ ∗ .VO[ξ] (fst ∘ vπ) d' ∗
+      ⌜(S d' ≤ d)%nat ∧ snd ∘ vπ = (.$ ξ)⌝ ∗ .VO[ξ] (fst ∘ vπ) d' ∗
       &{κ} (∃vπ' d', l ↦∗: ty.(ty_own) vπ' d' tid ∗ ⧖(S d') ∗ .PC[ξ] vπ' d');
     ty_shr vπ d κ' tid l := [S d' := d] ∃(l': loc) ξ, ⌜snd ∘ vπ ./ [ξ]⌝ ∗
       &frac{κ'}(λ q', l ↦{q'} #l') ∗ &frac{κ'} (λ q, q:[ξ]) ∗
